tests/elab/simproc_timeout.lean
@@ -23,8 +23,20 @@ end Std.Data.Nat.Basic
 
 section Mathlib.Logic.Equiv.Defs
 
-def Equiv.sigmaEquivProd (α β : Type _) : (Σ _ : α, β) ≃ α × β :=
-  ⟨fun a => ⟨a.1, a.2⟩, fun a => ⟨a.1, a.2⟩, fun _ => rfl, fun _ => rfl⟩
+structure Equiv (α : Sort _) (β : Sort _) where
+  protected toFun : α → β
+  protected invFun : β → α
+
+infixl:25 " ≃ " => Equiv
+
+namespace Equiv
+
+protected def symm (e : α ≃ β) : β ≃ α := ⟨e.invFun, e.toFun⟩
+
+def sigmaEquivProd (α β : Type _) : (Σ _ : α, β) ≃ α × β :=
+  ⟨fun a => ⟨a.1, a.2⟩, fun a => ⟨a.1, a.2⟩⟩
+
+end Equiv
 
 end Mathlib.Logic.Equiv.Defs
 
@@ -314,7 +326,7 @@ def ofNatCode : Nat → Code
   | _ => zero -- garbage value!
 
 instance instDenumerable : Denumerable Code :=
-  mk' ⟨encodeCode, ofNatCode, sorry, sorry⟩
+  mk' ⟨encodeCode, ofNatCode⟩
 
 open Primrec
 
